\documentclass[12pt,a4paper]{article}
\usepackage[utf8]{inputenc}
\usepackage[english]{babel}
\usepackage{amsmath}
\usepackage{amsfonts}
\usepackage{amssymb}
\usepackage[left=2cm,right=2cm,top=2cm,bottom=2cm]{geometry}
\author{Jiejia Xu}
\begin{document}

\[
T \sim \mathrm{exponential}(\lambda)
\]
\[
P(T \leq t) = 1- e^{-\lambda t} \quad (t\geq 0)
\]
\[
P(T > t) = e^{-\lambda t} \quad (t\geq 0)
\]

\[
f_T(t) = \begin{cases}
\lambda e^{-\lambda t} & (t \geq 0) \\
0 & (t < 0)
\end{cases}
\]

\[
P(T > t + s |T > t) = e^{-\lambda s}
\]

\[
T \sim \mathrm{exponential}(\lambda) \quad S \sim \mathrm{exponential}(\mu)
\]
\[
P(\min(T,S) > t) = e^{-(\lambda + \mu)t}
\]

\[
P(S<T) = \int_0^{\infty} f_S(s)P(T>s)ds = \frac{\mu}{\lambda+\mu}
\]

\[
T_i \sim \mathrm{exponential}(\lambda_i)
\]

\[
P(T_i = \min(T_1,T_2, \cdots, T_n)) = \frac{\lambda_i}{\lambda_1+\lambda_2 + \cdots + \lambda_n}
\]

\[
T_i \sim \mathrm{exponential}(\lambda)
\]
\[
S_n = T_1 + T_2 + \cdots + T_n
\]
\[
f_{S_n}(t) = \lambda e^{-\lambda t} \frac{(\lambda t)^{n-1}}{(n-1)!} \quad (t \geq 0)
\]

\[
f_{S_{n+1}}(t) = \int_0^t f_{S_n}(s)f_{T}(t-s)ds
\]

\[
N(t) = \max\{n: S_n \leq t\}
\]

\[
P(N(t) = n) = \int_0^t f_{S_n}(s)P(S_{n+1} > t-s)ds=  \frac{(\lambda t)^n}{n!}e^{-\lambda t}
\]

\[
N(t) \sim \mathrm{Poisson}(\lambda t)
\]

\[
X_i \sim \mathrm{Poisson}(\lambda_i)
\]

\[
P(X_1+X_2 = n) = \sum_{i = 0}^n P(X_1 = i)P(X_2 = n-i) = \frac{(\lambda_1+\lambda_2)^n}{n!}e^{-(\lambda_1+\lambda_2)}
\]

\[
N(t+s) - N(s) \sim \mathrm{Poisson}(\lambda t)
\]

\[
n \rightarrow \infty \quad \mathrm{binomial(n,\lambda/n)} \rightarrow \mathrm{Poisson}(\lambda) 
\]

\end{document}